fix some soundness proof in ConcreteHoare

core/ConcreteHoare.v
@@ -20,12 +20,26 @@ Notation P4Int := (P4Int.t tags_t).
 Notation P4String := (P4String.t tags_t).
 Notation signal := (@signal tags_t).
 Notation assertion := (@assertion tags_t).
+Notation arg_assertion := (@arg_assertion tags_t).
+Notation ret_assertion := (@ret_assertion tags_t).
 
 Context `{@Target tags_t (@Expression tags_t)}.
 
 Variable ge : (@genv tags_t).
 Variable inst_m : (@inst_mem tags_t).
 (* Variable this : path. *)
+
+Record post_assertion := mk_post_assertion {
+  post_continue :> assertion;
+  post_return : ret_assertion * assertion
+}.
+
+Definition to_shallow_post_assertion (p : path) (post : post_assertion) : Hoare.post_assertion :=
+  match post with 
+  | mk_post_assertion a_continue a_return =>
+      Hoare.mk_post_assertion (to_shallow_assertion p a_continue)
+        (fun vret st => ret_to_shallow_assertion (fst a_return) vret /\ to_shallow_assertion p (snd a_return) st)
+  end.
 
 Definition hoare_expr (pre : assertion) (expr : Expression) (v : Val) : Prop :=
   eval_expr ge pre expr = Some v.
@@ -62,8 +76,8 @@ Proof.
   eapply eval_write_sound; try eassumption.
 Qed.
 
-Inductive hoare_stmt : path -> assertion -> (@Statement tags_t) -> assertion -> Prop :=
-  | hoare_stmt_assignment : forall p pre tags lhs rhs typ post lv v,
+Inductive hoare_stmt : path -> assertion -> (@Statement tags_t) -> post_assertion -> Prop :=
+  | hoare_stmt_assignment : forall p pre tags lhs rhs typ (post : post_assertion) lv v,
       hoare_lexpr p pre lhs lv ->
       is_valid_field pre lv ->
       hoare_expr pre rhs v ->
@@ -73,9 +87,10 @@ Inductive hoare_stmt : path -> assertion -> (@Statement tags_t) -> assertion -> 
 Lemma hoare_stmt_sound : forall p pre stmt post,
   wellformed pre ->
   hoare_stmt p pre stmt post ->
-  Hoare.hoare_stmt ge inst_m p (to_shallow_assertion p pre) stmt (to_shallow_assertion p post).
+  Hoare.deep_hoare_stmt ge inst_m p (to_shallow_assertion p pre) stmt (to_shallow_post_assertion p post).
 Proof.
   intros * H_wellformed H_hoare_stmt.
+  apply deep_hoare_stmt_intro.
   induction H_hoare_stmt.
   - hnf. intros. pinv @exec_stmt.
     + repeat lazymatch goal with
@@ -83,23 +98,18 @@ Proof.
       | H : hoare_expr _ _ _ |- _ => apply hoare_expr_sound with (p := p) in H; only 2 : assumption
       | H : hoare_write _ _ _ _ |- _ => eapply hoare_write_sound with (p := p) in H; only 2 : assumption
       end.
-      specialize (H0 _ _ _ H4 H15).
-      specialize (H2 _ _ H4 H16); subst v0.
+      specialize (H0 _ _ _ H4 H16) as [? H0]; subst sig0.
+      specialize (H2 _ _ H4 H15); subst v0.
       eapply exec_write_congruent in H17. 3 : apply H0. 2 : { eapply state_is_valid_field_sound, is_valid_field_sound; eassumption. }
-      specialize (H3 _ _ H4 H17). sfirstorder.
+      specialize (H3 _ _ H4 H17). simpl. destruct post; sfirstorder.
     + pinv @exec_call; pinv hoare_expr.
-    + pinv @exec_call; pinv hoare_expr.
-    + lazymatch goal with
-      | H : hoare_lexpr _ _ _ _ |- _ => apply hoare_lexpr_sound in H
-      end.
-      unfold Hoare.hoare_lexpr in H0. hauto lq: on.
 Qed.
 
-Inductive hoare_block : path -> assertion -> (@Block tags_t) -> assertion -> Prop :=
-  | hoare_block_nil : forall p pre post tags,
+Inductive hoare_block : path -> assertion -> (@Block tags_t) -> post_assertion -> Prop :=
+  | hoare_block_nil : forall p pre (post : post_assertion) tags,
       implies pre post ->
       hoare_block p pre (BlockEmpty tags) post
-  | hoare_block_cons : forall p pre stmt rest mid post,
+  | hoare_block_cons : forall p pre stmt rest mid (post : post_assertion),
       hoare_stmt p pre stmt mid ->
       wellformed mid ->
       hoare_block p mid rest post ->
@@ -108,19 +118,14 @@ Inductive hoare_block : path -> assertion -> (@Block tags_t) -> assertion -> Pro
 Lemma hoare_block_sound : forall p pre block post,
   wellformed pre ->
   hoare_block p pre block post ->
-  Hoare.hoare_block ge inst_m p (to_shallow_assertion p pre) block (to_shallow_assertion p post).
+  Hoare.deep_hoare_block ge inst_m p (to_shallow_assertion p pre) block (to_shallow_post_assertion p post).
 Proof.
   intros * H_wellformed H_hoare_block.
   induction H_hoare_block.
-  - hnf. intros. pinv @exec_block.
-    split; only 1 : constructor.
-    eapply implies_sound; eassumption.
+  - constructor.
+    destruct post. intros st ?; eapply implies_sound; eassumption.
   - apply hoare_stmt_sound in H0; only 2 : assumption.
-    hnf. intros. pinv @exec_block.
-    + specialize (H0 _ _ _ H2 H9).
-      specialize (IHH_hoare_block H1 _ _ _ (proj2 H0) H12).
-      auto.
-    + specialize (H0 _ _ _ H2 H9). hauto.
+    destruct mid; econstructor; eauto.
 Qed.
 
 End ConcreteHoare.
